README.md
@@ -1,0 +1,25 @@
+# Lean tutorial
+
+This is the accompanying code for the invited lean tutorial held at DeFi Security Summit 2024 by Jakob von Raumer.
+
+It an abridged version of a Lean introductory talk at VSTT 2024 held by Joachim Breitner and Sebastian Ullrich, the material of which can be found [here](https://github.com/leanprover/vstte2024).
+
+## Synopsis
+
+* `Syntax.lean` defines the syntax of a small imperative language and embeds it into Lean.
+* `Eval.lean` defines an evaluation of the expressions of that language.
+* `Optimize.lean` provides a very simple optimization on these expressions and proves that it is consistent with the evaluation.
+* `BigStep.lean` defines a big step semantics for the language and proves some simple facts about it.
+
+## Ideas for Exercises
+
+* Add more expressiveness to the language: More operations, unary operations.
+* Improve `optimize` to simplify `0 + x` to `x`, for example.
+* Prove that `optimize` is idempotent: `e.optimize.optimize = e`.
+* Add nice input syntax for `Env.get σ "x"` and `Env.set`, e.g. `σ[[x]]` and `σ[[x := e]]` and update some of the proof statements.
+* Write an optimizer for `Stmt` which optimizes every expression.
+* Verify more complex programs! 
+Hint:
+
+Rephrase statements so that the three arguments to `BigStep` are variables, so that `induction` works. You can do that using a helper theorem that you finally apply, or explore the `generalize` tactic.
+
